IntroEffects/SmallStep.lean
@@ -5,8 +5,6 @@ import IntroEffects.LocallyNameless
   and prove its determinism.
 -/
 
-open Computation Value
-
 /--
   Returns the `OpClause` with name `name`.
 
@@ -38,41 +36,39 @@ inductive Step : Computation → Computation → Prop
     Since `body` is assumed to have one dangling bvar,
     we instantiate it with `v` to get the substitution.
  -/
-| beta v body : Step (app (lam body) v) (instantiateComp v body)
+| beta v body : Step (.app (.lam body) v) (instantiateComp v body)
 /-- `(recfun f x. body) v ⤳ body[recfun f x. body/f, v/x]
 
   Since `body` is assumed to have two dangling bvars,
   we replace the outermost one with a reference to the function itself
   and the inner one with the given argumetn `v`.
 -/
-| recBeta v body : Step (app (recfun body) v) (instantiate2 (recfun body) v body)
+| recBeta v body : Step (.app (.recfun body) v) (instantiate2 (.recfun body) v body)
 /-- `if True then c₁ else c₂ ⤳ c₁` -/
-| iteTrue c₁ c₂ : Step (ite (bool true) c₁ c₂) c₁
+| iteTrue c₁ c₂ : Step (.ite (.bool true) c₁ c₂) c₁
 /-- `if False then c₁ else c₂ ⤳ c₂` -/
-| iteFalse c₁ c₂ : Step (ite (bool false) c₁ c₂) c₂
+| iteFalse c₁ c₂ : Step (.ite (.bool false) c₁ c₂) c₂
 /--  If `c₁ ⤳ c₁'`, then `do x ← c₁ in c₂ ⤳ do x ← c₁' in c₂` -/
-| bindStep c₁ c₁' c₂ (h : Step c₁ c₁') : Step (bind c₁ c₂) (bind c₁' c₂)
+| bindStep c₁ c₁' c₂ (h : Step c₁ c₁') : Step (.bind c₁ c₂) (.bind c₁' c₂)
 /-- `do x ← return v in c ⤳ c[v/x]`
 
     Since `c` is the second argument to bind,
     we assume that it has one dangling bvar
     and so we instantiate it with `v` to get the substitution.
 -/
-| bindReturn v c : Step (bind (.ret v) c) (instantiateComp v c)
+| bindReturn v c : Step (.bind (.ret v) c) (instantiateComp v c)
 /-- `do x ← op(v; y.body) in c ⤳ op(v; y. do x ← body in c)`-/
-| bindOp op v body c : Step (bind (opCall op v body) c) (opCall op v (bind body c))
+| bindOp op v body c : Step (.bind (.opCall op v body) c) (.opCall op v (.bind body c))
 /-- If `c₁ ⤳ c₂`, then `with h handle c₁ ⤳ with h handle c₂` -/
-| handleInner h c₁ c₂ (h₁ : Step c₁ c₂) : Step (.handle (hdl h) c₁) (.handle (hdl h) c₂)
+| handleInner h c₁ c₂ (h₁ : Step c₁ c₂) : Step (.handle (.hdl h) c₁) (.handle (.hdl h) c₂)
 /-- `with h handle (return v) ⤳ retBody[v/x]`
 
     Since `retBody` is the return clause of a handler,
     we assume that it has one dangling bvar
     and so we instantiate it with `v` to get the substitution.
 -/
-| handleReturn h v retBody (hr : h.ret? = some retBody) :
-  Step (.handle (hdl h) (.ret v)) (instantiateComp v retBody)
-| handleReturnMiss h v (hr : h.ret? = none) :
-  Step (.handle (hdl h) (.ret v)) (.ret v)
+| handleReturn h v :
+  Step (.handle (.hdl h) (.ret v)) (instantiateComp v h.ret)
 /-- `with h handle op(v; y.body) ⤳ c[v/x, (y ↦ with h handle body)/k]`
 
     Since `c` is the body of an `OpClause`,
@@ -84,7 +80,7 @@ inductive Step : Computation → Computation → Prop
 -/
 | handleOpHit h op v body c (hop : h.lookup op = some ⟨op, c⟩) :
   Step (.handle (.hdl h) (.opCall op v body))
-    (instantiate2 v (lam (.handle (.hdl h) body)) c)
+    (instantiate2 v (.lam (.handle (.hdl h) body)) c)
 /-- `with h handle op(v; y.body) ⤳ op(v; y. with h handle body)`
 
     Since `body` is the body of an `opCall`,
@@ -93,7 +89,7 @@ inductive Step : Computation → Computation → Prop
     which means no substitution or instantiating is needed.
 -/
 | handleOpMiss h op v body (hop : h.lookup op = none) :
-  Step (.handle (.hdl h) (.opCall op v body)) (opCall op v (.handle (.hdl h) body))
+  Step (.handle (.hdl h) (.opCall op v body)) (.opCall op v (.handle (.hdl h) body))
 /--
   `join s₁ s₂ ⤳ return (str(strAppend s₁ s₂))`
 -/
@@ -105,7 +101,7 @@ inductive Step : Computation → Computation → Prop
 /--
   `snd pair(v₁, v₂) ⤳ return v₂`
 -/
-| sndStep v₁ v₂ : Step (.snd (pair v₁ v₂)) (.ret v₂)
+| sndStep v₁ v₂ : Step (.snd (.pair v₁ v₂)) (.ret v₂)
 | add v₁ v₂ : Step (.add (.num v₁) (.num v₂)) (.ret (.num (v₁ + v₂)))
 | sub v₁ v₂ : Step (.sub (.num v₁) (.num v₂)) (.ret (.num (v₁ - v₂)))
 | max v₁ v₂ : Step (.max (.num v₁) (.num v₂)) (.ret (.num (Max.max v₁ v₂)))
