IntroEffects/Type.lean
@@ -1,0 +1,142 @@
+import Std
+import IntroEffects.Expr
+
+mutual
+
+/--
+  The possible types for a value.
+-/
+inductive ValueTy where
+| bool
+| function : ValueTy → ComputationTy → ValueTy
+| handler : ComputationTy → ComputationTy → ValueTy
+
+/--
+  The type of a computation is the type of the value it returns
+  as well as the operations it can possibly call.
+-/
+inductive ComputationTy where
+| mk (returnTy : ValueTy) (Δ : List String)
+end
+
+notation A "!" Δ => ComputationTy.mk A Δ
+
+/--
+  The type of either a value or computation.
+-/
+inductive Ty where
+| val : ValueTy → Ty
+| comp : ComputationTy → Ty
+
+instance : Coe ValueTy Ty where
+  coe := .val
+instance : Coe ComputationTy Ty where
+  coe := .comp
+
+/--
+  An expression that is either a value or computation.
+-/
+inductive Expr where
+| val : Value → Expr
+| comp : Computation → Expr
+
+instance : Coe Value Expr where
+  coe := .val
+instance : Coe Computation Expr where
+  coe := .comp
+
+abbrev OpSignature := Std.TreeMap String (ValueTy × ValueTy)
+abbrev Ctx := List ValueTy
+
+def OpSignature.inputType (σ : OpSignature) (s : String)
+  (h : s ∈ σ := by grind) := σ.get s h |>.1
+def OpSignature.outputType (σ : OpSignature) (s : String)
+  (h : s ∈ σ := by grind) := σ.get s h |>.2
+
+/--
+  Find the `n`th type in the context
+-/
+def lookup : Ctx → Nat → Option ValueTy
+| [], _ => none
+| τ::_, 0 => some τ
+| _::Γ, n+1 => lookup Γ n
+
+notation "(" x " : " A ")" " ∈ " Γ => lookup Γ x = some A
+
+/--
+  `HasType σ Γ e T` means that `Γ ⊢ e : T`
+  with `σ` being the fixed types of all possible operation calls.
+-/
+inductive HasType (σ : OpSignature) : Ctx → Expr → Ty → Prop where
+/--
+ If `(x : A) ∈ Γ` then `Γ ⊢ x : A`
+-/
+| var x A : ((x : A) ∈ Γ) → HasType σ Γ (Value.var (.bvar x)) A
+/--
+  `Γ ⊢ True : bool` and `Γ ⊢ False : bool`
+-/
+| bool b : HasType σ Γ (Value.bool b) ValueTy.bool
+/--
+  If `Γ, x : A ⊢ c : C`, then `Γ ⊢ (fun x => c) : A → C`
+-/
+| lam A (c : Computation) (C : ComputationTy) :
+  HasType σ (A :: Γ) c C → HasType σ Γ (Value.lam c) (ValueTy.function A C)
+/--
+  If `Γ, x : A ⊢ cᵣ : B!Δ'`, `(opᵢ : Aᵢ → Bᵢ) ∈ Σ`,
+  `Γ, x : Aᵢ, k : Bᵢ → B!Δ' ⊢ cᵢ : B!Δ'`, and `Δ \ {opᵢ} ⊆ Δ'`,
+  then
+  `Γ ⊢ handler {return x ↦ cr, ops := [op₁(x, k) ↦ c₁, ⋯, opₙ(x, k) ↦ cₙ]} : A!Δ ⇒ B!Δ'`
+-/
+| handler (cr : Computation) :
+  HasType σ (A :: Γ) cr (B ! Δ') → -- `Γ, x : A ⊢ cᵣ : B!Δ'`
+  (h: ∀opClause ∈ ops, opClause.op ∈ σ) → -- `(opᵢ : Aᵢ → Bᵢ) ∈ Σ`
+  (∀mem : opClause ∈ ops,
+    let Aᵢ := σ.inputType opClause.op
+    let Bᵢ := σ.outputType opClause.op
+    let k := ValueTy.function Bᵢ (B ! Δ')
+    HasType σ (k :: Aᵢ :: Γ) opClause.body (B ! Δ')
+  ) → -- `Γ, x : Aᵢ, k : Bᵢ → B!Δ' ⊢ cᵢ : B!Δ'`
+  (Δ.removeAll (ops.map (·.op)) ⊆ Δ') → -- `Δ \ {opᵢ} ⊆ Δ'`
+  HasType σ Γ (Value.hdl (Handler.mk cr ops))
+    (ValueTy.handler (A ! Δ) (B ! Δ'))
+| ret (v : Value) Δ (A : ValueTy) : HasType σ Γ v A →
+  HasType σ Γ (Computation.ret v) (A ! Δ)
+/--
+  If `(op : Aop → Bop) ∈ Σ`, `Γ ⊢ v : Aop`, `Γ, y : Bop ⊢ c : A!Δ`, and `op ∈ Δ`
+  then `Γ ⊢ op(v; fun y ↦ c) : A!Δ`
+
+-/
+| op (v : Value) (c : Computation) :
+  (h : name ∈ σ) → -- `(op : Aop → Bop) ∈ Σ`
+  HasType σ Γ v (σ.inputType name) → -- `Γ ⊢ v : Aop`
+  HasType σ (σ.outputType name :: Γ) c (A ! Δ) → -- `Γ, y : Bop ⊢ c : A!Δ`
+  (name ∈ Δ) → -- `op ∈ Δ`
+  HasType σ Γ (Computation.opCall name v c) (A ! Δ)
+/--
+  If `Γ ⊢ c₁ : A!Δ` and `Γ, x : A ⊢ c₂ : B!Δ`
+  then `Γ ⊢ do x ← c₁ in c₂ : B!Δ`
+-/
+| bind (c₁ c₂ : Computation):
+  HasType σ Γ c₁ (A ! Δ) → HasType σ (A :: Γ) c₂ (B ! Δ) →
+  HasType σ Γ (Computation.bind c₁ c₂) (B ! Δ)
+/--
+  If `Γ ⊢ v₁ : A → C` and `Γ ⊢ v₂ : A`
+  then `Γ ⊢ v₁ v₂ : C`
+-/
+| app (v₁ v₂ : Value) :
+  HasType σ Γ v₁ (ValueTy.function A C) → HasType σ Γ v₂ A →
+  HasType σ Γ (Computation.app v₁ v₂) C
+/--
+  If `Γ ⊢ v : bool`, `Γ ⊢ c₁ : C`, and `Γ ⊢ c₂ : C`
+  then `Γ ⊢ if v then c₁ else c₂ : C`
+-/
+| ite (v : Value) (c₁ c₂ : Computation) :
+  HasType σ Γ v ValueTy.bool → HasType σ Γ c₁ C → HasType σ Γ c₂ C →
+  HasType σ Γ (Computation.ite v c₁ c₂) C
+/--
+  If `Γ ⊢ v : C ⇒ D` and `Γ : c : C`
+  then `Γ ⊢ with v handle c : D`
+-/
+| handle (v : Value) (c : Computation) :
+  HasType σ Γ v (ValueTy.handler C D) → HasType σ Γ c C →
+  HasType σ Γ (Computation.handle v c) D
